code/mpfr/MPFR.Add1sp1.fst
@@ -59,6 +59,8 @@ let mpfr_add1sp1_any_post_cond a b c h0 s h1 =
     (rb_def r p = (v s.rb <> 0)) /\
     (sb_def r p = (v s.sb <> 0)))
 
+(* The following inlined functions have abundant inputs,
+ * which are used for simplify the specifications *)
 inline_for_extraction val mpfr_add1sp1_gt_branch1:
     a:mpfr_struct -> b:mpfr_struct -> c:mpfr_struct ->
     ap:buffer mp_limb_t -> bp:buffer mp_limb_t -> cp:buffer mp_limb_t ->
@@ -174,18 +176,17 @@ let mpfr_add1sp1_eq a b c ap bp cp bx p sh =
     mk_state sh bx rb sb
 
 inline_for_extraction val mpfr_add1sp1_any:
-    a:mpfr_ptr -> b:mpfr_ptr -> c:mpfr_ptr ->
+    a:mpfr_ptr -> b:mpfr_ptr -> c:mpfr_ptr -> ap:buffer mp_limb_t ->
     p:mpfr_reg_prec_t -> Stack state
     (requires (fun h ->
-        mpfr_live h a /\ mpfr_live h b /\ mpfr_live h c /\
+        mpfr_live h a /\ mpfr_live h b /\ mpfr_live h c /\ ap == (as_struct h a).mpfr_d /\
         mpfr_add1sp1_any_pre_cond (as_struct h a) (as_struct h b) (as_struct h c) p h))
     (ensures  (fun h0 s h1 ->
         mpfr_add1sp1_any_post_cond (as_struct h0 a) (as_struct h0 b) (as_struct h0 c) h0 s h1))
 
-let mpfr_add1sp1_any a b c p =
+let mpfr_add1sp1_any a b c ap p =
     let bx = mpfr_GET_EXP b in
     let cx = mpfr_GET_EXP c in
-    let ap = mpfr_MANT a in
     let bp = mpfr_MANT b in
     let cp = mpfr_MANT c in
     let sh = I64.(gmp_NUMB_BITS -^ p) in
@@ -195,10 +196,11 @@ let mpfr_add1sp1_any a b c p =
     else mpfr_add1sp1_gt a.(0ul) c.(0ul) b.(0ul) ap cp bp cx bx p sh
 
 (* rounding specifications *)
-inline_for_extraction val mpfr_add_one_ulp: a:mpfr_ptr -> rnd_mode:mpfr_rnd_t ->
-                             sh:mpfr_reg_prec_t -> bx:mpfr_exp_t -> Stack i32
+inline_for_extraction val mpfr_add_one_ulp:
+    a:mpfr_ptr -> ap:buffer mp_limb_t -> rnd_mode:mpfr_rnd_t ->
+    sh:mpfr_reg_prec_t -> bx:mpfr_exp_t -> Stack i32
     (requires (fun h -> 
-    mpfr_live h a /\ length (as_struct h a).mpfr_d = 1 /\
+    mpfr_live h a /\ length (as_struct h a).mpfr_d = 1 /\ ap == (as_struct h a).mpfr_d /\
     normal_cond h a /\ mpfr_PREC_COND (I64.v (as_struct h a).mpfr_prec) /\
     sh = I64.(gmp_NUMB_BITS -^ (as_struct h a).mpfr_prec) /\
     bx = (as_struct h a).mpfr_exp /\ mpfr_EXP_COND (I64.v bx)))
@@ -207,9 +209,8 @@ inline_for_extraction val mpfr_add_one_ulp: a:mpfr_ptr -> rnd_mode:mpfr_rnd_t ->
     mpfr_round2_cond (add_one_ulp (as_normal h0 a)) rnd_mode (as_fp h1 a) /\
     I32.v t = mpfr_add1sp1_add_one_ulp_ternary_spec (as_normal h0 a) rnd_mode))
 
-let mpfr_add_one_ulp a rnd_mode sh bx =
+let mpfr_add_one_ulp a ap rnd_mode sh bx =
     let h0 = ST.get() in
-    let ap = mpfr_MANT a in
     ap.(0ul) <- ap.(0ul) +%^ (mpfr_LIMB_ONE <<^ (int64_to_uint32 sh));
     if ap.(0ul) =^ 0uL then begin
         ap.(0ul) <- mpfr_LIMB_HIGHBIT;
@@ -245,22 +246,23 @@ let mpfr_add_one_ulp a rnd_mode sh bx =
         mpfr_RET (mpfr_SIGN a)
     end
 
-inline_for_extraction val mpfr_add1sp1_round: a:mpfr_ptr -> rnd_mode:mpfr_rnd_t -> st:state -> Stack i32
+inline_for_extraction val mpfr_add1sp1_round:
+    a:mpfr_ptr -> ap:buffer mp_limb_t -> rnd_mode:mpfr_rnd_t -> st:state -> Stack i32
     (requires (fun h -> mpfr_live h a /\ length (as_struct h a).mpfr_d = 1 /\ normal_cond h a /\
-    (let high = {as_normal h a with exp = I64.v st.bx} in
-    let p = high.prec in
-    as_val h (as_struct h a).mpfr_d * pow2 (high.len - 64) = high.limb /\
-    I64.v st.sh = I64.v gmp_NUMB_BITS - p /\
-    mpfr_EXP_COND (I64.v st.bx))))
+        ap == (as_struct h a).mpfr_d /\
+        (let high = {as_normal h a with exp = I64.v st.bx} in
+        let p = high.prec in
+        as_val h (as_struct h a).mpfr_d * pow2 (high.len - 64) = high.limb /\
+        I64.v st.sh = I64.v gmp_NUMB_BITS - p /\
+        mpfr_EXP_COND (I64.v st.bx))))
     (ensures  (fun h0 t h1 -> 
-    mpfr_live h1 a /\ mpfr_modifies a h0 h1 /\ mpfr_valid_cond h1 a /\
-    (let high = {as_normal h0 a with exp = I64.v st.bx} in
-    mpfr_round2_cond (mpfr_add1sp1_round_spec high (st.rb <> 0uL) (st.sb <> 0uL) rnd_mode)
-                     rnd_mode (as_fp h1 a) /\
-    I32.v t = mpfr_add1sp1_ternary_spec high (st.rb <> 0uL) (st.sb <> 0uL) rnd_mode)))
+        mpfr_live h1 a /\ mpfr_modifies a h0 h1 /\ mpfr_valid_cond h1 a /\
+        (let high = {as_normal h0 a with exp = I64.v st.bx} in
+        mpfr_round2_cond (mpfr_add1sp1_round_spec high (st.rb <> 0uL) (st.sb <> 0uL) rnd_mode)
+                          rnd_mode (as_fp h1 a) /\
+        I32.v t = mpfr_add1sp1_ternary_spec high (st.rb <> 0uL) (st.sb <> 0uL) rnd_mode)))
 
-let mpfr_add1sp1_round a rnd_mode st =
-    let ap = mpfr_MANT a in
+let mpfr_add1sp1_round a ap rnd_mode st =
     let a0 = ap.(0ul) in
     let h0 = ST.get() in
     mpfr_SET_EXP a st.bx; // Maybe set it later in truncate and add_one_ulp?
@@ -272,10 +274,10 @@ let mpfr_add1sp1_round a rnd_mode st =
         if (st.rb =^ 0uL || (st.sb =^ 0uL && 
 	                   ((a0 &^ (mpfr_LIMB_ONE <<^ (int64_to_uint32 st.sh))) =^ 0uL))) then
 	    mpfr_RET (mpfr_NEG_SIGN (mpfr_SIGN a))
-	else mpfr_add_one_ulp a rnd_mode st.sh st.bx
+	else mpfr_add_one_ulp a ap rnd_mode st.sh st.bx
     else if mpfr_IS_LIKE_RNDZ rnd_mode (mpfr_IS_NEG a) then
         mpfr_RET (mpfr_NEG_SIGN (mpfr_SIGN a))
-    else mpfr_add_one_ulp a rnd_mode st.sh st.bx
+    else mpfr_add_one_ulp a ap rnd_mode st.sh st.bx
 
 (* specifications for mpfr_add1sp1 *)
 val mpfr_add1sp1: a:mpfr_ptr -> b:mpfr_ptr -> c:mpfr_ptr ->
@@ -305,7 +307,8 @@ val mpfr_add1sp1: a:mpfr_ptr -> b:mpfr_ptr -> c:mpfr_ptr ->
 
 let mpfr_add1sp1 a b c rnd_mode p =
     let h0 = ST.get() in
-    let st = mpfr_add1sp1_any a b c p in
+    let ap = mpfr_MANT a in
+    let st = mpfr_add1sp1_any a b c ap p in
     let h1 = ST.get() in
     lemma_reveal_modifies_1 (mpfr_MANT a) h0 h1;
     lemma_intro_modifies_2 a (mpfr_MANT a) h0 h1;
@@ -317,7 +320,7 @@ let mpfr_add1sp1 a b c rnd_mode p =
 	mpfr_modifies_trans_lemma a h0 h1 h2;
 	t
     end else begin
-        let t = mpfr_add1sp1_round a rnd_mode st in
+        let t = mpfr_add1sp1_round a ap rnd_mode st in
 	let h2 = ST.get() in
 	mpfr_add1sp1_round_post_cond_lemma (add1sp_exact (as_reg_fp h0 b) (as_reg_fp h0 c)) (I64.v (as_struct h0 a).mpfr_prec) (as_normal_ h1 ({as_struct h1 a with mpfr_exp = st.bx})) (st.rb <> 0uL) (st.sb <> 0uL) rnd_mode (I32.v t) (as_fp h2 a);
 	mpfr_modifies_trans_lemma a h0 h1 h2;
